Tidy up CakeML itree semantics proofs

cakeml-semantics/cakeml_semanticsProofScript.sml
@@ -3,11 +3,13 @@ open HolKernel Parse boolLib bossLib BasicProvers dep_rewrite;
 open optionTheory relationTheory pairTheory listTheory arithmeticTheory;
 open lem_pervasives_extraTheory libTheory namespaceTheory astTheory
      ffiTheory semanticPrimitivesTheory smallStepTheory evaluatePropsTheory;
-open io_treeTheory cakeml_semanticsTheory pure_miscTheory;
+open io_treeTheory pure_miscTheory
+     cakeml_semanticsTheory cakeml_semanticsPropsTheory;
 
 val _ = new_theory "cakeml_semanticsProof";
 
-(* TODO use evaluatePropsTheory and semanticPrimitivesPropsTheory *)
+
+(******************** Useful simplifications ********************)
 
 (* Deliberately no `application_def` here *)
 val smallstep_ss = simpLib.named_rewrites "smallstep_ss" [
@@ -21,353 +23,12 @@ val itree_ss = simpLib.named_rewrites "itree_ss" [
     cakeml_semanticsTheory.continue_def,
     cakeml_semanticsTheory.return_def,
     cakeml_semanticsTheory.push_def,
-    cakeml_semanticsTheory.estep_def
+    cakeml_semanticsTheory.estep_def,
+    get_ffi_def
     ];
 
 
-(****************************************)
-
-
-(* Copied from CakeML *)
-Theorem cml_application_thm:
-  ∀op env s vs c.
-    application op env s vs c =
-    if op = Opapp then
-      case do_opapp vs of
-      | NONE => Eabort Rtype_error
-      | SOME (env,e) => Estep (env,s,Exp e,c)
-    else
-      case do_app s op vs of
-      | NONE => Eabort Rtype_error
-      | SOME (v1,Rval v') => return env v1 v' c
-      | SOME (v1,Rerr (Rraise v)) => Estep (env,v1,Val v,(Craise (),env)::c)
-      | SOME (v1,Rerr (Rabort a)) => Eabort a
-Proof
-  rw[smallStepTheory.application_def] >> every_case_tac >> gvs[]
-QED
-
-Theorem application_thm:
-  ∀op env s vs c.
-    application op env s vs c =
-    if op = Opapp then
-      case do_opapp vs of
-      | NONE => Etype_error
-      | SOME (env,e) => Estep (env,s,Exp e,c)
-    else if ∃n. op = FFI n then (
-      case op of FFI n => (
-        case vs of
-          [Litv (StrLit conf); Loc lnum] => (
-            case store_lookup lnum s of
-              SOME (W8array ws) =>
-                if n = "" then Estep (env, s, Val $ Conv NONE [], c)
-                else Effi n (MAP (λc. n2w $ ORD c) (EXPLODE conf)) ws lnum env s c
-            | _ => Etype_error)
-        | _ => Etype_error)
-      | _ => ARB)
-    else
-      case do_app s op vs of
-      | NONE => Etype_error
-      | SOME (v1,Rval v') => return env v1 v' c
-      | SOME (v1,Rraise v) => Estep (env,v1,Val v,(Craise,env)::c)
-Proof
-  reverse $ rw[application_def] >> gvs[SF itree_ss] >>
-  TOP_CASE_TAC >> gvs[]
-QED
-
-
-(****************************************)
-(* Adapt CakeML's RTC definitions to our more functional definitions *)
-
-
-Definition step_n_cml_def:
-  step_n_cml 0 e = e ∧
-  step_n_cml (SUC n) (Estep st) = step_n_cml n (e_step st) ∧
-  step_n_cml _ e = e
-End
-
-Theorem step_n_same[simp]:
-  ∀n.
-    step_n n Edone = Edone ∧
-    step_n n Etype_error = Etype_error ∧
-    step_n n (Effi s ws1 ws2 n env st cs) = (Effi s ws1 ws2 n env st cs) ∧
-    step_n_cml n Estuck = Estuck ∧
-    step_n_cml n (Eabort a) = Eabort a
-Proof
-  Cases >> rw[step_n_def, step_n_cml_def]
-QED
-
-Theorem step_n_cml_alt_def:
-  step_n_cml 0 e = e ∧
-  step_n_cml (SUC n) e = (
-    case step_n_cml n e of
-    | Estep st => e_step st
-    | e => e)
-Proof
-  rw[step_n_cml_def] >>
-  qid_spec_tac `e` >> qid_spec_tac `n` >>
-  Induct >> Cases >> rewrite_tac[step_n_cml_def] >> simp[]
-QED
-
-Theorem step_n_cml_add:
-  ∀a b. step_n_cml (a + b) e = step_n_cml a (step_n_cml b e)
-Proof
-  Induct >> rw[step_n_cml_def] >>
-  simp[ADD_CLAUSES, step_n_cml_alt_def]
-QED
-
-Theorem e_step_reln_eq_step_n_cml:
-  e_step_reln^* st1 st2 ⇔
-  ∃n. step_n_cml n (Estep st1) = Estep st2
-Proof
-  reverse $ eq_tac >> rw[] >> pop_assum mp_tac
-  >- (
-    map_every qid_spec_tac [`st2`,`st1`,`n`] >>
-    Induct >> rw[step_n_cml_alt_def] >>
-    every_case_tac >> gvs[] >>
-    rw[Once relationTheory.RTC_CASES2] >> disj2_tac >>
-    last_x_assum $ irule_at Any >> gvs[e_step_reln_def]
-    )
-  >- (
-    Induct_on `RTC e_step_reln` >> rw[]
-    >- (qexists_tac `0` >> gvs[step_n_cml_def])
-    >- (qexists_tac `SUC n` >> gvs[step_n_cml_def, e_step_reln_def])
-    )
-QED
-
-Definition is_halt_cml_def:
-  is_halt_cml (Estep (env, st_ffi, Val v, [])) = T ∧
-  is_halt_cml (Estep (env, st_ffi, Val v, [Craise (), env'])) = T ∧
-  is_halt_cml (Eabort a) = T ∧
-  is_halt_cml _ = F
-End
-
-Definition step_to_halt_cml_def:
-  step_to_halt_cml e =
-    case some n. is_halt_cml (step_n_cml n e) of
-    | NONE => NONE
-    | SOME n => SOME $ step_n_cml n e
-End
-
-Theorem small_eval_eq_step_n_cml:
-  (small_eval env st_ffi e cs (st_ffi', Rval v) ⇔
-  ∃n env'.
-    step_n_cml n (Estep (env, st_ffi, Exp e, cs)) =
-      (Estep (env', st_ffi', Val v, []))) ∧
-  (small_eval env st_ffi e cs (st_ffi', Rerr (Rraise v)) ⇔
-  ∃n env' env''.
-    step_n_cml n (Estep (env, st_ffi, Exp e, cs)) =
-      (Estep (env', st_ffi', Val v, [(Craise (), env'')]))) ∧
-  ((∃st_ffi'. small_eval env st_ffi e cs (st_ffi', Rerr (Rabort a))) ⇔
-  ∃n env' env''.
-    step_n_cml n (Estep (env, st_ffi, Exp e, cs)) = Eabort a)
-Proof
-  reverse $ rw[small_eval_def, e_step_reln_eq_step_n_cml]
-  >- (
-    eq_tac >> rw[]
-    >- (qexists_tac `SUC n` >> gvs[step_n_cml_alt_def]) >>
-    Induct_on `n` >> gvs[step_n_cml_alt_def] >>
-    every_case_tac >> gvs[] >> rw[PULL_EXISTS] >>
-    PairCases_on `p` >> goal_assum drule >> simp[]
-    ) >>
-  eq_tac >> rw[] >> ntac 2 $ goal_assum drule
-QED
-
-Triviality Estep_is_halt_imp_e_step_neq_Estep:
-  is_halt_cml (Estep st) ⇒ ∀st'. e_step st ≠ Estep st'
-Proof
-  PairCases_on `st` >> rw[] >>
-  Cases_on `st3` >> Cases_on `st4` >> gvs[is_halt_cml_def]
-  >- simp[e_step_def, SF smallstep_ss] >>
-  PairCases_on `h` >>
-  Cases_on `h0` >> Cases_on `t` >> gvs[is_halt_cml_def] >>
-  simp[e_step_def, SF smallstep_ss]
-QED
-
-Triviality Estep_is_halt_imp_step_n_neq_Estep:
-  is_halt_cml st ⇒ ∀st'. step_n_cml (SUC n) st ≠ Estep st'
-Proof
-  Cases_on `st` >> gvs[is_halt_cml_def] >>
-  PairCases_on `p` >>
-  Cases_on `p3` >> gvs[is_halt_cml_def] >>
-  Cases_on `p4` >> gvs[is_halt_cml_def]
-  >- (gvs[step_n_cml_def, e_step_def, SF smallstep_ss, is_halt_cml_def]) >>
-  PairCases_on `h` >> Cases_on `h0` >> gvs[is_halt_cml_def] >>
-  Cases_on `t` >> gvs[is_halt_cml_def] >>
-  gvs[step_n_cml_def, e_step_def, SF smallstep_ss, is_halt_cml_def]
-QED
-
-Triviality Estep_is_halt_imp_not_is_halt_step_n_cml:
-  is_halt_cml (Estep st) ⇒ ¬ is_halt_cml (step_n_cml (SUC n) (Estep st))
-Proof
-  PairCases_on `st` >> gvs[is_halt_cml_def] >>
-  Cases_on `st3` >> gvs[is_halt_cml_def] >>
-  Cases_on `st4` >> gvs[is_halt_cml_def]
-  >- (gvs[step_n_cml_def, e_step_def, SF smallstep_ss, is_halt_cml_def]) >>
-  PairCases_on `h` >> Cases_on `h0` >> gvs[is_halt_cml_def] >>
-  Cases_on `t` >> gvs[is_halt_cml_def] >>
-  gvs[step_n_cml_def, e_step_def, SF smallstep_ss, is_halt_cml_def]
-QED
-
-Theorem is_halt_cml_step_n_cml_eq:
-  ∀n m e.
-    is_halt_cml (step_n_cml n e) ∧
-    is_halt_cml (step_n_cml m e)
-  ⇒ step_n_cml n e = step_n_cml m e
-Proof
-  rw[] >> wlog_tac `n < m` [`n`,`m`]
-  >- (Cases_on `n = m` >> gvs[]) >>
-  imp_res_tac LESS_STRONG_ADD >> gvs[] >>
-  gvs[step_n_cml_add |> ONCE_REWRITE_RULE[ADD_COMM]] >>
-  Cases_on `step_n_cml n e` >> gvs[] >>
-  imp_res_tac Estep_is_halt_imp_not_is_halt_step_n_cml
-QED
-
-Theorem step_n_add:
-  ∀a b. step_n (a + b) e = step_n a (step_n b e)
-Proof
-  Induct >> rw[step_n_def] >>
-  simp[ADD_CLAUSES, step_n_alt_def]
-QED
-
-Theorem is_halt_step_n_eq:
-  ∀n m e.
-    is_halt (step_n n e) ∧
-    is_halt (step_n m e)
-  ⇒ step_n n e = step_n m e
-Proof
-  rw[] >> wlog_tac `n < m` [`n`,`m`]
-  >- (Cases_on `n = m` >> gvs[]) >>
-  imp_res_tac LESS_STRONG_ADD >> gvs[] >>
-  gvs[step_n_add |> ONCE_REWRITE_RULE[ADD_COMM]] >>
-  Cases_on `step_n n e` >> gvs[is_halt_def, step_n_def]
-QED
-
-Theorem small_eval_eq_step_to_halt_cml:
-  (small_eval env st_ffi e cs (st_ffi', Rval v) ⇔
-  ∃env'.
-    step_to_halt_cml (Estep (env, st_ffi, Exp e, cs)) =
-      SOME (Estep (env', st_ffi', Val v, []))) ∧
-  (small_eval env st_ffi e cs (st_ffi', Rerr (Rraise v)) ⇔
-  ∃env' env''.
-    step_to_halt_cml (Estep (env, st_ffi, Exp e, cs)) =
-      SOME (Estep (env', st_ffi', Val v, [(Craise (), env'')]))) ∧
-  ((∃st_ffi'. small_eval env st_ffi e cs (st_ffi', Rerr (Rabort a))) ⇔
-  ∃env' env''.
-    step_to_halt_cml (Estep (env, st_ffi, Exp e, cs)) = SOME (Eabort a))
-Proof
-  rw[small_eval_eq_step_n_cml, step_to_halt_cml_def] >> eq_tac >>
-  DEEP_INTRO_TAC some_intro >> rw[] >> gvs[]
-  >- metis_tac[is_halt_cml_step_n_cml_eq, is_halt_cml_def]
-  >- (
-    pop_assum $ qspec_then `n` assume_tac >>
-    CCONTR_TAC >> gvs[is_halt_cml_def]
-    )
-  >- goal_assum drule
-  >- metis_tac[is_halt_cml_step_n_cml_eq, is_halt_cml_def]
-  >- (
-    pop_assum $ qspec_then `n` assume_tac >>
-    CCONTR_TAC >> gvs[is_halt_cml_def]
-    )
-  >- goal_assum drule
-  >- metis_tac[is_halt_cml_step_n_cml_eq, is_halt_cml_def]
-  >- (
-    pop_assum $ qspec_then `n` assume_tac >>
-    CCONTR_TAC >> gvs[is_halt_cml_def]
-    )
-  >- goal_assum drule
-QED
-
-Theorem application_not_Edone:
-  application op env st vs cs ≠ Edone
-Proof
-  rw[application_thm] >>
-  every_case_tac >> gvs[SF itree_ss]
-QED
-
-Theorem estep_to_Edone:
-  estep (env, st, ev, cs) = Edone ⇔
-  (∃v. ev = Val v ∧ cs = []) ∨
-  (∃v env'. ev = Val v ∧ cs = [Craise, env'])
-Proof
-  reverse $ eq_tac
-  >- (rw[] >> gvs[SF itree_ss]) >>
-  Cases_on `ev` >> gvs[estep_def]
-  >- (
-    Cases_on `e` >> gvs[estep_def, SF itree_ss] >>
-    every_case_tac >> gvs[] >> rw[application_not_Edone]
-    ) >>
-  Cases_on `cs` >> gvs[SF itree_ss] >>
-  PairCases_on `h` >> Cases_on `h0` >> gvs[SF itree_ss] >>
-  every_case_tac >> gvs[]
-  >- (
-    rename1 `Capp _ _ es` >>
-    Cases_on `es` >> gvs[SF itree_ss, application_not_Edone]
-    )
-  >- (
-    rename1 `Cmat l _` >> Cases_on `l` >> gvs[SF itree_ss] >>
-    PairCases_on `h` >> gvs[SF itree_ss] >> every_case_tac >> gvs[]
-    )
-  >- (
-    rename1 `Ccon _ _ es` >> Cases_on `es` >> gvs[SF itree_ss] >>
-    every_case_tac >> gvs[]
-    )
-QED
-
-Theorem application_not_Estuck:
-  application op env st_ffi vs cs ≠ Estuck
-Proof
-  rw[cml_application_thm] >>
-  EVERY_CASE_TAC >> gvs[SF smallstep_ss]
-QED
-
-Theorem e_step_to_Estuck:
-  e_step (env, st_ffi, ev, cs) = Estuck ⇔
-  (∃v. ev = Val v ∧ cs = []) ∨
-  (∃v env'. ev = Val v ∧ cs = [Craise (), env'])
-Proof
-  reverse $ eq_tac
-  >- (rw[] >> gvs[SF smallstep_ss]) >>
-  gvs[e_step_def] >> CASE_TAC >> gvs[]
-  >- (every_case_tac >> gvs[SF smallstep_ss, application_not_Estuck]) >>
-  Cases_on `cs` >> gvs[SF smallstep_ss] >>
-  every_case_tac >> gvs[application_not_Estuck]
-QED
-
-Theorem e_diverges_eq_step_to_halt_cml:
-  e_diverges env st_ffi e ⇔ step_to_halt_cml (Estep (env, st_ffi, Exp e, [])) = NONE
-Proof
-  rw[step_to_halt_cml_def, e_diverges_def, e_step_reln_eq_step_n_cml] >>
-  simp[PULL_EXISTS] >>
-  eq_tac >> rw[] >> gvs[e_step_reln_def]
-  >- (
-    DEEP_INTRO_TAC some_intro >> rw[] >>
-    Induct_on `x` >> rw[] >> gvs[step_n_cml_alt_def, is_halt_cml_def] >>
-    CASE_TAC >> gvs[is_halt_def] >>
-    PairCases_on `p` >> rename1 `Estep (a, b, c, d)` >>
-    last_assum drule >> strip_tac >> gvs[] >> rename1 `Estep (f, g, h, i)` >>
-    last_x_assum $ qspecl_then [`f`,`g`,`h`,`i`,`SUC x`] assume_tac >>
-    gvs[step_n_cml_alt_def] >>
-    metis_tac[Estep_is_halt_imp_e_step_neq_Estep]
-    )
-  >- (
-    last_x_assum mp_tac >>
-    DEEP_INTRO_TAC some_intro >> rw[] >>
-    first_assum $ qspec_then `n` assume_tac >>
-    first_x_assum $ qspec_then `SUC n` assume_tac >> gvs[step_n_cml_alt_def] >>
-    Cases_on `e_step (env', s', e', c')` >> gvs[is_halt_cml_def]
-    >- (PairCases_on `p` >> simp[]) >>
-    gvs[e_step_to_Estuck, is_halt_cml_def]
-    )
-QED
-
-
-(****************************************)
-
-
-Inductive result_rel:
-  result_rel (Rval v) (Rval v) ∧
-  result_rel (Rraise v) (Rerr $ Rraise v)
-End
+(******************** Simpler lemmas ********************)
 
 (* Takes 30s *)
 Theorem do_app_rel:
@@ -382,32 +43,6 @@ Proof
     gvs[do_app_def, result_rel_cases, store_alloc_def]
     )
 QED
-
-Inductive ctxt_frame_rel:
-  ctxt_frame_rel Craise (Craise ()) ∧
-  ctxt_frame_rel (Chandle pes) (Chandle () pes) ∧
-  ctxt_frame_rel (Capp op vs es) (Capp op vs () es) ∧
-  ctxt_frame_rel (Clog lop e) (Clog lop () e) ∧
-  ctxt_frame_rel (Cif e1 e2) (Cif () e1 e2) ∧
-  ctxt_frame_rel (Cmat_check pes v) (Cmat_check () pes v) ∧
-  ctxt_frame_rel (Cmat pes v) (Cmat () pes v) ∧
-  ctxt_frame_rel (Clet vopt e) (Clet vopt () e) ∧
-  ctxt_frame_rel (Ccon idopt vs es) (Ccon idopt vs () es) ∧
-  ctxt_frame_rel (Ctannot ty) (Ctannot () ty) ∧
-  ctxt_frame_rel (Clannot ls) (Clannot () ls)
-End
-
-Definition ctxt_rel_def:
-  ctxt_rel cs1 cs2 =
-    LIST_REL (λ(c1,env1) (c2,env2). ctxt_frame_rel c1 c2 ∧ env1 = env2) cs1 cs2
-End
-
-Inductive step_result_rel:
-  (ctxt_rel cs1 cs2 ⇒
-    step_result_rel (Estep (env, st, ev, cs1)) (Estep (env, (st, ffi), ev, cs2))) ∧
-  step_result_rel Edone Estuck ∧
-  step_result_rel Etype_error (Eabort $ Rtype_error)
-End
 
 (* Takes 20s *)
 Theorem application_rel:
@@ -433,15 +68,6 @@ Proof
     )
 QED
 
-Triviality application_FFI_results:
-  (application (FFI s) env st vs cs = Etype_error) ∨
-  (application (FFI s) env st vs cs = Estep (env, st, Val $ Conv NONE [], cs)) ∨
-  ∃conf ws lnum.
-    (application (FFI s) env st vs cs) = Effi s conf ws lnum env st cs
-Proof
-  rw[application_def] >> every_case_tac >> gvs[]
-QED
-
 Theorem application_rel_FFI_type_error:
   application (FFI s) env st vs cs1 = Etype_error ⇔
   application (FFI s) env (st, ffi) vs cs2 = Eabort Rtype_error
@@ -464,197 +90,8 @@ Proof
   every_case_tac >> gvs[] >> rw[] >> gvs[ffi_state_component_equality]
 QED
 
-Triviality application_eq_Effi_fields:
-  application op env st vs cs = Effi s conf ws lnum env' st' cs' ⇒
-  op = FFI s ∧ env = env' ∧ st = st' ∧ cs' = cs ∧
-  ∃conf'.
-    vs = [Litv $ StrLit conf'; Loc lnum] ∧
-    conf = MAP (λc. n2w $ ORD c) (EXPLODE conf')
-Proof
-  Cases_on `op` >> simp[application_def, SF itree_ss] >>
-  every_case_tac >> gvs[] >> rw[]
-QED
 
-Theorem application_rel_FFI:
-  application (FFI s) env st vs cs1 = Effi s conf ws lnum env st cs1 ⇒
-    store_lookup lnum st = SOME $ W8array ws ∧
-    application (FFI s) env (st, ffi) vs cs2 =
-      case ffi.oracle s ffi.ffi_state conf ws of
-      | Oracle_return ffi' ws' =>
-          if LENGTH ws' ≠ LENGTH ws then
-            Eabort $ Rffi_error $ Final_event s conf ws FFI_failed
-          else
-            Estep (env,
-              (LUPDATE (W8array ws') lnum st,
-               ffi with <|
-                  ffi_state := ffi';
-                  io_events := ffi.io_events ++ [IO_event s conf (ZIP (ws,ws'))]
-                  |>),
-              Val $ Conv NONE [], cs2)
-      | Oracle_final outcome =>
-          Eabort $ Rffi_error $ Final_event s conf ws outcome
-Proof
-  simp[application_def] >>
-  ntac 6 (TOP_CASE_TAC >> gvs[]) >>
-  gvs[store_lookup_def] >>
-  ntac 2 (TOP_CASE_TAC >> gvs[]) >> rw[] >> gvs[] >>
-  simp[smallStepTheory.application_def, semanticPrimitivesTheory.do_app_def] >>
-  simp[store_lookup_def, call_FFI_def] >>
-  qmatch_goalsub_abbrev_tac `foo l` >>
-  reverse $ Cases_on `foo l` >> gvs[] >>
-  IF_CASES_TAC >> gvs[store_assign_def, store_v_same_type_def, SF smallstep_ss]
-QED
-
-Theorem application_rel_FFI':
-  application (FFI s) env (st, ffi) vs cs2 ≠ Eabort Rtype_error ⇒
-  (∃conf lnum ws.
-    vs = [Litv $ StrLit conf; Loc lnum] ∧
-    store_lookup lnum st = SOME $ W8array ws ∧
-    application (FFI s) env st vs cs1 =
-      Effi s (MAP (λc. n2w $ ORD c) (EXPLODE conf)) ws lnum env st cs1) ∨
-  (s = "" ∧
-  application (FFI s) env st vs cs1 = Estep (env, st, Val $ Conv NONE [], cs1))
-Proof
-  rw[smallStepTheory.application_def, semanticPrimitivesTheory.do_app_def] >>
-  every_case_tac >> gvs[application_def] >>
-  IF_CASES_TAC >> gvs[]
-QED
-
-Theorem do_app_ffi_changed:
-  do_app (st, ffi) op vs = SOME ((st', ffi'), res) ∧
-  ffi ≠ ffi' ⇒
-  ∃s conf lnum ws ffi_st ws'.
-    op = FFI s ∧
-    vs = [Litv (StrLit conf); Loc lnum] ∧
-    store_lookup lnum st = SOME (W8array ws) ∧
-    s ≠ "" ∧
-    ffi.oracle s ffi.ffi_state (MAP (λc. n2w $ ORD c) (EXPLODE conf)) ws =
-      Oracle_return ffi_st ws' ∧
-    LENGTH ws = LENGTH ws' ∧
-    st' = LUPDATE (W8array ws') lnum st ∧
-    ffi'.oracle = ffi.oracle ∧
-    ffi'.ffi_state = ffi_st ∧
-    ffi'.io_events =
-      ffi.io_events ++
-        [IO_event s (MAP (λc. n2w $ ORD c) (EXPLODE conf)) (ZIP (ws,ws'))]
-Proof
-  simp[semanticPrimitivesTheory.do_app_def] >>
-  every_case_tac >> gvs[store_alloc_def, store_assign_def] >>
-  strip_tac >> gvs[call_FFI_def] >>
-  every_case_tac >> gvs[]
-QED
-
-Theorem do_app_ffi_unchanged:
-  ∀st ffi op vs st' ffi' res.
-    (∀s. op ≠ FFI s) ∧
-    do_app (st, ffi) op vs = SOME ((st', ffi'), res)
-  ⇒ ffi = ffi'
-Proof
-  rpt gen_tac >>
-  simp[semanticPrimitivesTheory.do_app_def] >>
-  every_case_tac >> gvs[store_alloc_def]
-QED
-
-Theorem application_ffi_unchanged:
-  ∀op env st ffi vs cs env' st' ffi' ev cs'.
-    (∀s. op ≠ FFI s) ∧
-    application op env (st, ffi) vs cs = Estep (env', (st', ffi'), ev, cs')
-  ⇒ ffi = ffi'
-Proof
-  rpt gen_tac >>
-  rw[cml_application_thm, SF smallstep_ss]
-  >- (every_case_tac >> gvs[]) >>
-  qspecl_then [`st`,`ffi`,`op`,`vs`] assume_tac do_app_ffi_unchanged >>
-  every_case_tac >> gvs[]
-QED
-
-Theorem e_step_ffi_changed:
-  e_step (env, (st, ffi), ev, cs) = Estep (env', (st', ffi'), ev', cs') ∧
-  ffi ≠ ffi' ⇒
-  ∃ s conf lnum ccs ws ffi_st ws'.
-    ev = Val (Litv (StrLit conf)) ∧
-    cs = (Capp (FFI s) [Loc lnum] () [], env') :: ccs ∧
-    store_lookup lnum st = SOME (W8array ws) ∧
-    s ≠ "" ∧
-    ffi.oracle s ffi.ffi_state (MAP (λc. n2w $ ORD c) (EXPLODE conf)) ws =
-      Oracle_return ffi_st ws' ∧
-    LENGTH ws = LENGTH ws' ∧
-    ev' = Val (Conv NONE []) ∧
-    cs' = ccs ∧
-    st' = LUPDATE (W8array ws') lnum st ∧
-    ffi'.oracle = ffi.oracle ∧
-    ffi'.ffi_state = ffi_st ∧
-    ffi'.io_events =
-      ffi.io_events ++
-        [IO_event s (MAP (λc. n2w $ ORD c) (EXPLODE conf)) (ZIP (ws,ws'))]
-Proof
-  simp[e_step_def] >>
-  every_case_tac >> gvs[SF smallstep_ss]
-  >- (
-    strip_tac >> rename1 `application op _ _ _ _` >>
-    Cases_on `∀s. op ≠ FFI s` >> gvs[]
-    >- (irule application_ffi_unchanged >> rpt $ goal_assum drule) >>
-    gvs[smallStepTheory.application_def, semanticPrimitivesTheory.do_app_def]
-    ) >>
-  every_case_tac >> gvs[] >>
-  rename1 `application op _ _ _ _` >>
-  (
-    strip_tac >> Cases_on `∀s. op ≠ FFI s` >> gvs[]
-    >- (drule_all application_ffi_unchanged >> gvs[]) >>
-    gvs[smallStepTheory.application_def,
-        semanticPrimitivesTheory.do_app_def, call_FFI_def] >>
-    every_case_tac >> gvs[SF smallstep_ss, store_lookup_def, store_assign_def]
-  )
-QED
-
-Theorem e_step_ffi_changed_imp_estep_eq_Effi:
-  e_step (env, (st, ffi), ev, cs2) = Estep (env', (st', ffi'), ev', cs2') ∧
-  ffi ≠ ffi' ∧
-  ctxt_rel cs1 cs2 ⇒
-  ∃ s conf lnum ccs ws.
-    ev = Val (Litv (StrLit conf)) ∧
-    cs1 = (Capp (FFI s) [Loc lnum] [], env') :: ccs ∧
-    store_lookup lnum st = SOME (W8array ws) ∧
-    estep (env, st, ev, cs1) =
-      Effi s (MAP (λc. n2w $ ORD c) (EXPLODE conf)) ws lnum env' st ccs
-Proof
-  rw[] >> drule_all e_step_ffi_changed >> rw[] >>
-  gvs[ctxt_rel_def] >> pairarg_tac >> gvs[ctxt_frame_rel_cases] >>
-  simp[estep_def, SF itree_ss, application_thm]
-QED
-
-Definition is_Effi_def:
-  is_Effi (Effi _ _ _ _ _ _ _) = T ∧
-  is_Effi _ = F
-End
-
-Theorem is_Effi_def:
-  is_Effi e ⇔ ∃ s ws1 ws2 n env st cs. e = Effi s ws1 ws2 n env st cs
-Proof
-  Cases_on `e` >> simp[is_Effi_def]
-QED
-
-Definition get_ffi_def:
-  get_ffi (Estep (env, (st, ffi), ev, cs)) = SOME ffi ∧
-  get_ffi _ = NONE
-End
-
-(****************************************)
-
-
-(* Play out a particular trace prefix from a given itree, modelling the
-   environment as an FFI oracle with associated FFI state (as in CakeML) *)
-Definition trace_prefix_def:
-  trace_prefix 0 (oracle, st) itree = ([], NONE) ∧
-  trace_prefix (SUC n) (oracle, st) (Ret r) = ([], SOME r) ∧
-  trace_prefix (SUC n) (oracle, st) (Vis (s, conf, ws) f) =
-    case oracle s st conf ws of
-    | Oracle_return st' ws' =>
-        let (io, res) = trace_prefix n (oracle, st) (f $ INR ws') in
-        (IO_event s conf (ZIP (ws,ws'))::io, res)
-    | Oracle_final outcome => trace_prefix n (oracle, st) (f $ INL outcome)
-End
-
+(******************** Relating non-FFI steps ********************)
 
 Theorem step_result_rel_single:
   ∀ea eb.
@@ -759,6 +196,70 @@ Proof
   unabbrev_all_tac >> gvs[get_ffi_def]
 QED
 
+
+(******************** Relating FFI steps ********************)
+
+Theorem application_rel_FFI:
+  application (FFI s) env st vs cs1 = Effi s conf ws lnum env st cs1 ⇒
+    store_lookup lnum st = SOME $ W8array ws ∧
+    application (FFI s) env (st, ffi) vs cs2 =
+      case ffi.oracle s ffi.ffi_state conf ws of
+      | Oracle_return ffi' ws' =>
+          if LENGTH ws' ≠ LENGTH ws then
+            Eabort $ Rffi_error $ Final_event s conf ws FFI_failed
+          else
+            Estep (env,
+              (LUPDATE (W8array ws') lnum st,
+               ffi with <|
+                  ffi_state := ffi';
+                  io_events := ffi.io_events ++ [IO_event s conf (ZIP (ws,ws'))]
+                  |>),
+              Val $ Conv NONE [], cs2)
+      | Oracle_final outcome =>
+          Eabort $ Rffi_error $ Final_event s conf ws outcome
+Proof
+  simp[application_def] >>
+  ntac 6 (TOP_CASE_TAC >> gvs[]) >>
+  gvs[store_lookup_def] >>
+  ntac 2 (TOP_CASE_TAC >> gvs[]) >> rw[] >> gvs[] >>
+  simp[smallStepTheory.application_def, semanticPrimitivesTheory.do_app_def] >>
+  simp[store_lookup_def, call_FFI_def] >>
+  qmatch_goalsub_abbrev_tac `foo l` >>
+  reverse $ Cases_on `foo l` >> gvs[] >>
+  IF_CASES_TAC >> gvs[store_assign_def, store_v_same_type_def, SF smallstep_ss]
+QED
+
+Theorem application_rel_FFI':
+  application (FFI s) env (st, ffi) vs cs2 ≠ Eabort Rtype_error ⇒
+  (∃conf lnum ws.
+    vs = [Litv $ StrLit conf; Loc lnum] ∧
+    store_lookup lnum st = SOME $ W8array ws ∧
+    application (FFI s) env st vs cs1 =
+      Effi s (MAP (λc. n2w $ ORD c) (EXPLODE conf)) ws lnum env st cs1) ∨
+  (s = "" ∧
+  application (FFI s) env st vs cs1 = Estep (env, st, Val $ Conv NONE [], cs1))
+Proof
+  rw[smallStepTheory.application_def, semanticPrimitivesTheory.do_app_def] >>
+  every_case_tac >> gvs[application_def] >>
+  IF_CASES_TAC >> gvs[]
+QED
+
+Theorem e_step_ffi_changed:
+  e_step (env, (st, ffi), ev, cs2) = Estep (env', (st', ffi'), ev', cs2') ∧
+  ffi ≠ ffi' ∧
+  ctxt_rel cs1 cs2 ⇒
+  ∃ s conf lnum ccs ws.
+    ev = Val (Litv (StrLit conf)) ∧
+    cs1 = (Capp (FFI s) [Loc lnum] [], env') :: ccs ∧
+    store_lookup lnum st = SOME (W8array ws) ∧
+    estep (env, st, ev, cs1) =
+      Effi s (MAP (λc. n2w $ ORD c) (EXPLODE conf)) ws lnum env' st ccs
+Proof
+  rw[] >> drule_all e_step_ffi_changed >> rw[] >>
+  gvs[ctxt_rel_def] >> pairarg_tac >> gvs[ctxt_frame_rel_cases] >>
+  simp[estep_def, SF itree_ss, application_thm]
+QED
+
 Theorem step_result_rel_single_FFI:
   ∀ea eb.
     step_result_rel (Estep ea) (Estep eb) ∧
@@ -794,13 +295,7 @@ Proof
   >- (rpt (CASE_TAC >> gvs[SF itree_ss]))
 QED
 
-Theorem step_result_rel_not_Effi:
-  ∀e1 e2. step_result_rel e1 e2 ⇒ ¬ is_Effi e1
-Proof
-  rw[step_result_rel_cases, is_Effi_def]
-QED
-
-Theorem e_step_ffi_same_imp_estep_neq_Effi:
+Theorem step_result_rel_single_FFI':
   (∀ffi. get_ffi (e_step e2) = SOME ffi ⇒ get_ffi (Estep e2) = SOME ffi) ∧
   (∀a. e_step e2 ≠ Eabort $ Rffi_error a) ∧
   step_result_rel (Estep e1) (Estep e2)
@@ -813,60 +308,7 @@ Proof
   rw[] >> gvs[]
 QED
 
-Triviality step_n_cml_eq_Estep:
-  ∀n e st.
-    step_n_cml n e = Estep st
-  ⇒ ∀m. m < n ⇒ ∃st'. step_n_cml m e = Estep st'
-Proof
-  Induct >> rw[step_n_cml_def] >>
-  Cases_on `e` >> gvs[step_n_cml_def] >>
-  Cases_on `m` >> gvs[step_n_cml_def]
-QED
-
-Theorem io_events_mono_e_step:
-  e_step e1 = Estep e2 ⇒
-  io_events_mono (SND $ FST $ SND e1) (SND $ FST $ SND e2)
-Proof
-  PairCases_on `e1` >> PairCases_on `e2` >> gvs[] >> rw[] >>
-  rename1 `e_step (env1,(st1,ffi1),ev1,cs1) = _ (env2,(st2,ffi2),ev2,cs2)` >>
-  Cases_on `ffi1 = ffi2` >- simp[io_events_mono_refl] >>
-  drule_all e_step_ffi_changed >> rw[] >> gvs[] >>
-  rw[io_events_mono_def]
-QED
-
-Theorem io_events_mono_step_n_cml:
-  ∀n e1 e2.
-    step_n_cml n (Estep e1) = Estep e2
-  ⇒ io_events_mono (SND $ FST $ SND e1) (SND $ FST $ SND e2)
-Proof
-  Induct >> rw[step_n_cml_alt_def] >>
-  irule io_events_mono_trans >>
-  last_x_assum $ irule_at Any >>
-  qspecl_then [`SUC n`,`Estep e1`,`e2`] mp_tac step_n_cml_eq_Estep >>
-  gvs[step_n_cml_alt_def] >>
-  disch_then $ qspec_then `n` mp_tac >> gvs[] >>
-  strip_tac >> gvs[] >>
-  irule io_events_mono_e_step >> simp[]
-QED
-
-Theorem step_n_cml_preserved_FFI:
-  ∀n e e'.
-    step_n_cml n e = Estep e' ∧ get_ffi (Estep e') = get_ffi e
-  ⇒ ∀m. m < n ⇒ get_ffi (step_n_cml m e) = get_ffi (Estep e')
-Proof
-  rw[] >> imp_res_tac LESS_STRONG_ADD >>
-  gvs[step_n_cml_add |> ONCE_REWRITE_RULE[ADD_COMM]] >> rename1 `SUC n` >>
-  Cases_on `step_n_cml m e` >> gvs[] >>
-  PairCases_on `p` >> rename1 `(env1,(st1,ffi1),ev1,cs1)` >>
-  Cases_on `e` >> gvs[] >>
-  PairCases_on `p` >> rename1 `_ = get_ffi $ _ (env,(st,ffi),ev,cs)` >>
-  PairCases_on `e'` >>
-  rename1 `step_n_cml (SUC _) _ = Estep (env2,(st2,ffi2),ev2,cs2)` >>
-  imp_res_tac io_events_mono_step_n_cml >> gvs[get_ffi_def] >>
-  imp_res_tac io_events_mono_antisym >> gvs[]
-QED
-
-Theorem step_n_ffi_same_imp_step_result_rel:
+Theorem step_result_rel_n':
   ∀n e1 e2.
     get_ffi (step_n_cml n (Estep e2)) = get_ffi (Estep e2) ∧
     step_result_rel (Estep e1) (Estep e2)
@@ -887,16 +329,12 @@ Proof
   Cases_on `e_step (env,(st,ffi),ev,cs2)` >> gvs[get_ffi_def] >>
   disch_then $ qspec_then `n` mp_tac >> simp[get_ffi_def] >> rw[] >> gvs[] >>
   first_assum $ once_rewrite_tac o single o GSYM >>
-  irule e_step_ffi_same_imp_estep_neq_Effi >>
+  irule step_result_rel_single_FFI' >>
   simp[get_ffi_def, step_result_rel_cases]
 QED
 
 
-
-
-
-
-(****************************************)
+(******************** interp ********************)
 
 Theorem interp_Ret_Termination:
   ctxt_rel cs1 cs2 ⇒
@@ -906,9 +344,8 @@ Theorem interp_Ret_Termination:
     (∃v st'. small_eval env (st, ffi) e cs2 ((st', ffi), Rerr $ Rraise v))
   )
 Proof
-  rw[interp_def] >> eq_tac >> rw[]
+  rw[Once interp] >> eq_tac >> rw[]
   >- (
-    gvs[Once cml_io_unfold_err] >>
     every_case_tac >> gvs[io_distinct, step_until_halt_def] >>
     pop_assum mp_tac >> DEEP_INTRO_TAC some_intro >> rw[] >> gvs[] >>
     reverse every_case_tac >> gvs[is_halt_def] >>
@@ -950,7 +387,7 @@ Proof
     pop_assum mp_tac >> impl_tac
     >- (
       irule step_result_rel_not_Effi >>
-      irule_at Any step_n_ffi_same_imp_step_result_rel >>
+      irule_at Any step_result_rel_n' >>
       qexists_tac `(env,(st,ffi),Exp e,cs2)` >>
       simp[get_ffi_def, step_result_rel_cases, ctxt_rel_def]
       ) >>
@@ -978,7 +415,7 @@ Proof
     pop_assum mp_tac >> impl_tac
     >- (
       irule step_result_rel_not_Effi >>
-      irule_at Any step_n_ffi_same_imp_step_result_rel >>
+      irule_at Any step_result_rel_n' >>
       qexists_tac `(env,(st,ffi),Exp e,cs2)` >>
       simp[get_ffi_def, step_result_rel_cases, ctxt_rel_def]
       ) >>
@@ -1004,9 +441,8 @@ Theorem interp_Ret_Error:
     ∃st'. small_eval env (st, ffi) e cs2 ((st', ffi), Rerr $ Rabort Rtype_error)
   )
 Proof
-  rw[interp_def] >> eq_tac >> rw[]
+  rw[Once interp] >> eq_tac >> rw[]
   >- (
-    gvs[Once cml_io_unfold_err] >>
     every_case_tac >> gvs[io_distinct, step_until_halt_def] >>
     pop_assum mp_tac >> DEEP_INTRO_TAC some_intro >> rw[] >> gvs[] >>
     every_case_tac >> gvs[is_halt_def] >>
@@ -1033,7 +469,7 @@ Proof
     pop_assum mp_tac >> impl_tac
     >- (
       irule step_result_rel_not_Effi >>
-      irule_at Any step_n_ffi_same_imp_step_result_rel >>
+      irule_at Any step_result_rel_n' >>
       qexists_tac `(env,(st,ffi),Exp e,cs2)` >>
       simp[get_ffi_def, step_result_rel_cases, ctxt_rel_def]
       ) >>
@@ -1045,7 +481,7 @@ Proof
       gvs[get_ffi_def] >> pop_assum mp_tac >> impl_tac >> rw[] >> gvs[is_halt_def] >>
       qsuff_tac `¬is_Effi (estep (env',st',e',cs1'))` >- gvs[is_Effi_def] >>
       irule step_result_rel_not_Effi >>
-      irule_at Any e_step_ffi_same_imp_estep_neq_Effi >>
+      irule_at Any step_result_rel_single_FFI' >>
       simp[step_result_rel_cases, PULL_EXISTS, ctxt_rel_def] >>
       goal_assum $ drule_at Any >> qexists_tac `ffi` >> simp[get_ffi_def]) >>
     DEEP_INTRO_TAC some_intro >> reverse $ rw[] >> gvs[]
@@ -1070,9 +506,8 @@ Theorem interp_Ret_SilentDivergence:
       get_ffi (Estep st2) = SOME ffi
   )
 Proof
-  rw[interp_def] >> eq_tac >> rw[]
+  rw[Once interp] >> eq_tac >> rw[]
   >- (
-    gvs[Once cml_io_unfold_err] >>
     every_case_tac >> gvs[io_distinct, step_until_halt_def] >>
     every_case_tac >> gvs[] >>
     pop_assum mp_tac >> DEEP_INTRO_TAC some_intro >> rw[] >> gvs[] >>
@@ -1099,16 +534,14 @@ Proof
     simp[step_n_alt_def, estep_def, SF itree_ss, is_halt_def]
     )
   >- (
-    rw[Once cml_io_unfold_err, step_until_halt_def] >>
+    rw[step_until_halt_def] >>
     DEEP_INTRO_TAC some_intro >> rw[] >> gvs[] >>
-    irule FALSITY >>
-    pop_assum mp_tac >>
-    simp[] >>
+    irule FALSITY >> pop_assum mp_tac >> simp[] >>
     pop_assum $ qspec_then `x` assume_tac >> gvs[] >>
     PairCases_on `st2` >> gvs[get_ffi_def] >>
     rename1 `¬is_halt_cml (Estep (env',(st',_),ev,cs2'))` >>
     qspecl_then [`x`,`(env,st,Exp e,cs1)`,`(env,(st,ffi),Exp e,cs2)`]
-      assume_tac step_n_ffi_same_imp_step_result_rel >>
+      assume_tac step_result_rel_n' >>
     gvs[step_result_rel_cases, get_ffi_def] >>
     simp[is_halt_def]
     )
